statement of join-exist client

examples/joining_existentials.v
@@ -1,7 +1,42 @@
-From iris.program_logic Require Import saved_one_shot.
+From iris.program_logic Require Import saved_one_shot hoare.
 From iris.barrier Require Import proof specification.
 From iris.heap_lang Require Import notation par.
 
-Definition client (eM eW1 eW2 : expr []) : expr [] :=
-  (let: "b" := newbarrier #() in (^^eM ;; ^signal '"b") ||
-                              ((^wait '"b" ;; ^^eW1) || (^wait '"b" ;; ^^eW2))).
+Definition client eM eW1 eW2 : expr [] :=
+  (let: "b" := newbarrier #() in (eM ;; ^signal '"b") ||
+                              ((^wait '"b" ;; eW1) || (^wait '"b" ;; eW2))).
+
+Section proof.
+Context (G : cFunctor).
+Context {Σ : gFunctors} `{!heapG Σ, !barrierG Σ, !oneShotG heap_lang Σ G}.
+Context (heapN N : namespace).
+Local Notation iProp := (iPropG heap_lang Σ).
+Local Notation X := (G iProp).
+
+Definition barrier_res γ (P : X → iProp) : iProp :=
+  (∃ x:X, one_shot_own γ x ★ P x)%I.
+
+
+Lemma worker_spec e γ l (P Q : X → iProp) (R : iProp) Φ :
+  R ⊢ (∀ x, {{ P x }} e {{ λ _, Q x }}) →
+  R ⊢ (recv heapN N l (barrier_res γ P) ★ (∀ v : val, barrier_res γ Q -★ Φ v )) →
+  R ⊢ WP ^wait (%l) ;; e {{ Φ }}.
+Proof.
+Abort.
+
+Context (P' : iProp) (P P1 P2 Q Q1 Q2 : X → iProp).
+Context {P_split : (∃ x:X, P x) ⊢ ((∃ x:X, P1 x) ★ (∃ x:X, P2 x))}.
+Context {Q_join  : ((∃ x:X, Q1 x) ★ (∃ x:X, Q2 x)) ⊢ (∃ x:X, Q x)}.
+
+Lemma client_spec eM eM' eW1 eW1' eW2 eW2' (R : iProp) :
+  eM' = wexpr' eM → eW1' = wexpr' eW1 → eW2' = wexpr' eW2 →
+  R ⊢ ({{ P' }} eM {{ λ _, ∃ x, P x }}) →
+  R ⊢ (∀ x, {{ P1 x }} eW1 {{ λ _, Q1 x }}) →
+  R ⊢ (∀ x, {{ P2 x }} eW2 {{ λ _, Q2 x }}) →
+  R ⊢ heap_ctx heapN →
+  R ⊢ WP client eM' eW1' eW2' {{ λ _, ∃ γ, barrier_res γ Q }}.
+Proof.
+Abort.
+  
+
+End proof.
